\input{defGn}
%%%%%%%%
\begin{document}
\title{Differential Geometry HW4}
\author{\asemail}
\maketitle
\def\t{T\!\!}%微分几何用切空间
\def\d{\,\mathrm{d}}
\def\f #1{\frac{\partial }{\partial {#1}}}%定义坐标切向量
%按照题号抄题并解答。
\begin{enumerate}
\isep[1em]

\prob
$(M,g)$ is a Rienmannian manifold. 
For $\theta \in T^*M$, the vector $\theta^\# \in TM$ is called the dual of $\theta$ if $$
g(\theta^\#,X)=\theta(X), \forall X\in TM.$$
Define the dual metric $g^*$ 
\begin{align*}
	g^*:\quad \otimes^2 T^*M &\to \r \\
	(\theta,\sigma) &\mapsto g(\theta^\#,\sigma^\#).
\end{align*}
If $g=g_{ij}\d x_i \d x_j$ in a local coordinate, calculate the coordinate components of $g^*$.
\soln
For coordinate dual vector $\d x_i$, assume $\d x_i^\#=A_{ik}\f{x_k}$ where the index $k$ appeared twice denote summation for $k$ according to Einstein summation convention. 
For any coordinate vector $\f{x_j}$, \begin{align*}
	g(\d x_i^\#, \f{x_j}) &= g(A_{ik}\f{x_k}, \f{x_j}) \\
	&= A_{ik}g(\f{x_k},\f{x_j}) \\
	&= A_{ik}g_{kj}; \\
	g(\d x_i^\#, \f{x_j}) &= \d x_i(\f{x_j}) \\
	&= \delta_{ij}.
\end{align*}
Thus $A_{ik}=g^{ik}$. Because \begin{align*}
	g^*(\d x_i,\d x_j) &= g(\d x_i^\#,\d x_j^\#) \\
	&= g(A_{ik}\f{x_k}, A_{jl}\f{x_l}) \\
	&= A_{ik}A_{jl}g(\f{x_k},\f{x_l}) \\
	&= g^{ik}g^{jl}g_{kl} \\
	&= g^{ij},
\end{align*}
we get $g^*=g^{ij} \f{x_i}\f{x_j}$.
\qed

\prob The map
\begin{align*}
	\phi:\quad S^2 &\to \r^4 \\
	(x,y,z) &\mapsto (\frac{x^2-y^2}{2},xy,yz,zx)
\end{align*}
is an immersion. $\phi$ induce a Rienmannian metric from the standard metric on $\r^4$, 
\begin{align*}
	\phi^* \d s^2 &= \d \phi_1^2+ \d \phi_2^2+ \d \phi_3^2+ \d \phi_4^2 \\
	&= (x \d x-y \d y)^2 + (y\d x+x\d y)^2 + (z\d y+y\d z)^2 + (x\d z+z\d x)^2 \\
	&= \d x^2 + \d y^2 + (x^2+y^2-2z^2)\d z^2.
\end{align*}
Calculate the Gauss curvature of $\phi^* \d s^2$.
\soln
Use $x^2+y^2+z^2=1$, \begin{align*}
	\phi^* \d s^2 &= (\d \sqrt{1-(y^2+z^2)})^2+\d y^2+ (1-z^2-2z^2)d z^2 \\
	&= (\frac{-y}{x}\d y+\frac{-z}{x}\d z)^2+\d y^2+ (1-3z^2)d z^2 \\
	&= \frac{y^2+x^2}{x^2} \d y^2 +\frac{yz}{x^2}\d y\d z +\frac{yz}{x^2}\d z\d y+ \frac{x^2+z^2-3x^2z^2}{x^2}\d z^2.
\end{align*}
Caution $x\neq 0$. The dual metric $g^*= (\phi^*g)^{ij}\f{x_i}\f{x_j}$, \begin{align*}
	(\phi^*g) &= \frac{1}{3z^2(x^2+y^2)-1} \begin{pmatrix}
		3z^2x^2+y^2-1 & yz \\
		yz & z^2-1
	\end{pmatrix} .
\end{align*}
Then $\theta_1=\d z, \theta_2=(1-z^2)\d y+yz\d z$ are two orthogonal dual vector on $S^2$ and \begin{align*}
	\d\theta_1 &=0, \\
	\d\theta_2 &= -2z\d z \d y+z\d y\d z \\
	&= 3z \d y\d z \\
	&= -\frac{3z}{1-z^2} \theta_1\wedge \theta_2.
\end{align*}
Solve the structure equation 
$$\left\{\begin{aligned}
	0 &=\omega_{12}\wedge \theta_2, \\
	-\frac{3z}{1-z^2} \theta_1\wedge \theta_2 &=-\omega_{12}\wedge \theta_1.
\end{aligned}\right. $$
We get $\omega_{12}= -\frac{3z}{1-z^2} \theta_2$, and \begin{align*}
	\d \omega_{12} &= -\frac{3(1-z^2)-3z(-2z)}{(1-z^2)^2}\d z\wedge \theta_2 \\
	&= -\frac{3+3z^2}{(1-z^2)^2}\d z\wedge \theta_2 \\
	&= -\frac{3+3z^2}{(1-z^2)^2} \theta_1\wedge \theta_2.
\end{align*}
The Gauss curvature of $(S^2, \phi^* g)$ is $K=\frac{3+3z^2}{(1-z^2)^2}$.
\qed

\par Use the \textbf{stereographic projection} $X(u,v)=\frac{1}{1+u^2+v^2}(2u,2v,u^2+v^2-1)$ with $z\neq 1$, \begin{align*}
	\phi^* \d s^2 &= \d x^2 + \d y^2 + (x^2+y^2-2z^2)\d z^2 \\
	&= (\d \frac{2u}{1+u^2+v^2})^2+(\d \frac{2v}{1+u^2+v^2})^2 +(1-3(\frac{u^2+v^2-1}{1+u^2+v^2})^2)(\d \frac{u^2+v^2-1}{1+u^2+v^2})^2 \\
	&= (\frac{2}{1+u^2+v^2}\d u + \frac{-2u}{(1+u^2+v^2)^2}(2u\d u+2v\d v))^2 \\
	&+ (\frac{2}{1+u^2+v^2}\d v+ \frac{-2v}{(1+u^2+v^2)^2}(2u\d u+2v\d v))^2 \\
	&+ (1-3(\frac{u^2+v^2-1}{1+u^2+v^2})^2)(\frac{2u\d u+2v\d v}{1+u^2+v^2}+ \frac{u^2+v^2-1}{(1+u^2+v^2)^2}(2u\d u+2v\d v))^2 \\
	&= (\frac{2(1-u^2+v^2)}{(1+u^2+v^2)^2}\d u + \frac{-4uv}{(1+u^2+v^2)^2}\d v)^2+ (\frac{2(1+u^2-v^2)}{(1+u^2+v^2)^2}\d v + \frac{-4uv}{(1+u^2+v^2)^2}\d u)^2 \\
	%&+ \frac{-2(u^2+v^2)^2+8(u^2+v^2)-2}{(1+u^2+v^2)^2}(\frac{4u(u^2+v^2)}{(1+u^2+v^2)^2}\d u+ \frac{4v(u^2+v^2)}{(1+u^2+v^2)^2}\d v)^2 \\
	&+ (1-3z^2)(\frac{4u(u^2+v^2)}{(1+u^2+v^2)^2}\d u+ \frac{4v(u^2+v^2)}{(1+u^2+v^2)^2}\d v)^2 \\
	&= ((\frac{-2z}{1+u^2+v^2}+y^2)\d u - xy\d v)^2+ ((\frac{-2z}{1+u^2+v^2}+x^2)\d v - xy\d u)^2 \\
	&+ (1-3z^2)(2x(z+\frac{1}{1+u^2+v^2})\d u+ 2y(z+\frac{1}{1+u^2+v^2})\d v)^2 \\
	&= ((z+z^2 +y^2)\d u - xy\d v)^2+ ((z+z^2+x^2)\d v - xy\d u)^2 \\
	&+ (1-3z^2)(x(z+1)\d u+ y(z+1)\d v)^2 \\
	&= ((z+z^2 +y^2)\d u - xy\d v)^2+ ((z+z^2+x^2)\d v - xy\d u)^2 \\
	&+ (1-3z^2)(x(z+1)\d u+ y(z+1)\d v)^2 \\
	&= (1+z-3x^2z^2)(1+z)\d u^2 -6xyz^2(1+z)^2\d u\d v +(1+z-3y^2z^2)(1+z)\d v^2 \\
	&= \begin{pmatrix}
	(1+z-3x^2z^2)(1+z) & -3xyz^2(1+z)^2 \\
	- 3xyz^2(1+z)^2 & (1+z-3y^2z^2)(1+z)
	\end{pmatrix}.\times \begin{pmatrix}
		\d u^2 & \d u \d v \\
		\d v\d u & \d v^2
	\end{pmatrix}.
\end{align*}
Use the other stereographic projection $Y(u,v)=\frac{1}{1+u^2+v^2}(2u,2v,1-u^2-v^2)$ where $(u,v)=\frac{(u,v)}{u^2+v^2}$ with $z\neq -1$, we get \begin{align*}
	\phi^* \d s^2 &= (1+z-3x^2z^2)(1+z)(\d \frac{u}{u^2+v^2})^2 \\
	&-6xyz^2(1+z)^2\d \frac{u}{u^2+v^2}\d \frac{v}{u^2+v^2} +(1+z-3y^2z^2)(1+z)(\d \frac{v}{u^2+v^2})^2 \\
	&= (1-z-3x^2z^2)(1-z)\d u^2 -6xyz^2(1-z)^2\d u\d v +(1-z-3y^2z^2)(1-z)\d v^2 \\
	&= \begin{pmatrix}
	(1-z-3x^2z^2)(1-z) & -3xyz^2(1-z)^2 \\
	- 3xyz^2(1-z)^2 & (1-z-3y^2z^2)(1-z)
	\end{pmatrix}.\times \begin{pmatrix}
		\d u^2 & \d u \d v \\
		\d v\d u & \d v^2
	\end{pmatrix}.
\end{align*}

\newpage
\prob 
Suppose $\{v_1,\cdots,v_n\},\{w_1,\cdots,w_n\}$ are two bases of an $n$-dimensional vector space $V$, and $$
(v_1,\cdots,v_n)=(w_1,\cdots,w_n)J.$$
Prove that $$
v_1\wedge v_2 \wedge \cdots \wedge v_n = \det{J} w_1\wedge w_2 \wedge \cdots \wedge w_n.$$
\soln
Use the Einstein summation convention since the summations are from $1$ to $n$, then $v_i= w_k J_{ki}$ for $1\leq i \leq n$. 
\begin{align*}
	v_1\wedge v_2 \wedge \cdots \wedge v_n &= w_{k_1}J_{k_1 1}\wedge w_{k_2}J_{k_2 2} \wedge \cdots \wedge w_{k_n}J_{k_n n} \\
	&= J_{k_11}J_{k_22}\cdots J_{k_nn} w_{k_1}\wedge w_{k_2} \wedge \cdots \wedge w_{k_n} \\
	&= \sum_{\sigma\in S_n} J_{\sigma(1)1}J_{\sigma(2)2}\cdots J_{\sigma(n)n} w_{\sigma(1)}\wedge w_{\sigma(2)} \wedge \cdots \wedge w_{\sigma(n)} \\
	&= \sum_{\sigma\in S_n} \delta(\sigma) J_{\sigma(1)1}J_{\sigma(2)2}\cdots J_{\sigma(n)n} w_1\wedge w_2 \wedge \cdots \wedge w_n \\
	&= \det{J} w_1\wedge w_2 \wedge \cdots \wedge w_n.
\end{align*}
\qed

\end{enumerate}
\end{document}